specs/frodo/test-64-AES/Spec.Frodo.Test.fsti
@@ -2,4 +2,4 @@ module Spec.Frodo.Test
 
 open FStar.All
 
-val test: unit -> ML unit
+val test: unit -> ML bool
